\documentclass[11pt]{article}

\input{./defs.tex}

\begin{document}

\hwtitle
  {Assignment 1}
  {Eric Wen} %% REPLACE THIS WITH YOUR NAME/ID

\problem{Problem 1}

\begin{enumerate}
\item $\fun{x}{x}$. Condition 1 is met.
\item $\fun{x}{y}$. Condition 1 is met.
\item $x$. Condition 2 is met.
\item $\fun{y}{\app{(\fun{y'}{\app{y'}{y'}})}{y}}$. Condition 1 is met.
\item $\app{(\fun{x}{\app{x}{x}})}{(\fun{x}{\app{x}{x}})}$. Condition 3 is met.
\item $b$. Condition 2 is met.
\item $\fun{y}{z}$. Condition 1 is met.
\end{enumerate}

\problem{Problem 3}

%Your answer goes here. Here's the dynamically-scoped untyped lambda calculus operational semantics as examples of writing inference rules.
%
%\begin{mathpar}
%\ir{V-Lam}{ \ }{\val{\fun{x}{e}}}
%
%\ir{D-Var}
%  {\ctx(x) = e}
%  {\dynJC{\steps{x}{e}}}
%
%\ir{D-App$_1$}
%  {\dynJC{\steps{e_1}{e_1'}}}
%  {\dynJC{\steps{\app{e_1}{e_2}}{\app{e_1'}{e_2}}}}
%
%\ir{D-App$_2$}
%  {\dynJ{\ctx, x \rightarrow e_2}{\steps{e_1}{e_1'}}}
%  {\dynJC{\steps{\app{(\fun{x}{e_1})}{e_2}}{\app{(\fun{x}{e_1'})}{e_2}}}}
%
%\ir{D-App$_3$}
%  {\val{e_1}}
%  {\dynJC{\steps{\app{(\fun{x}{e_1})}{e_2}}{e_1}}}
%\end{mathpar}

Step 1:

\begin{mathpar}
\ir{D-App$_2$}{
	\ir{D-App$_1$}{
		\ir{D-App$_3$}{
			\ir{D-Lam}{
			}{
				\val{
					\fun{\_}{x}
				}
			}
		}{
			\{
				x\rightarrow D
			\}
			\vdash
			\steps{
				\app{
					(\fun{x}{
						\fun{\_}{x}
					})
				}{L}
			}{
				\fun{\_}{x}
			}
		}
	}{
		\{
			x\rightarrow D
		\}
		\vdash
		\steps{
			\app{
				\app{
					(\fun{x}{
						\fun{\_}{x}
					})
				}{L}
			}{*}
		}{
			\app{
				(\fun{\_}{x})
			}{*}
		}
	}
}{
	\varnothing
	\vdash
	\steps{
		\app{
			(\fun{x}{
				\app{
					\app{
						(\fun{x}{
							\fun{\_}{x}
						})
					}{L}
				}{*}
			})
		}{D}
	}{
		\app{
			(\fun{x}{
				\app{
					(\fun{\_}{x})
				}{*}
			})
		}{D}
	}
}
\end{mathpar}

Step 2:

\begin{mathpar}
\ir{D-App$_2$}{
	\ir{D-App$_2$}{
		\ir{D-Var}{
			x\rightarrow D\in\{
				x\rightarrow D,
				\_\rightarrow *
			\}
		}{
			\{
				x\rightarrow D,
				\_\rightarrow *
			\}
			\vdash
			\steps{x}{D}
		}
	}{
		\{
			x\rightarrow D
		\}
		\vdash
		\steps{
			\app{
				(\fun{\_}{x})
			}{*}
		}{
			\app{
				(\fun{\_}{D})
			}{*}
		}
	}
}{
	\varnothing
	\vdash
	\steps{
		\app{
			(\fun{x}{
				\app{
					(\fun{\_}{x})
				}{*}
			})
		}{D}
	}{
		\app{
			(\fun{x}{
				\app{
					(\fun{\_}{D})
				}{*}
			})
		}{D}
	}
}
\end{mathpar}

Step 3:

\begin{mathpar}
\ir{D-App$_2$}{
	\ir{D-App$_2$}{
		\ir{D-App$_3$}{
			\val{D}
		}{
			\{
				x\rightarrow D,
				\_\rightarrow *
			\}
			\vdash
			\steps{
				\app{
					(\fun{\_}{D})
				}{*}
			}{D}
		}
	}{
		\{
			x\rightarrow D
		\}
		\vdash
		\steps{
			\fun{x}{
				\app{
					(\fun{\_}{D})
				}{*}
			}
		}{
			\fun{x}{D}
		}
	}
}{
	\varnothing
	\vdash
	\steps{
		\app{
			(\fun{x}{
				\app{
					(\fun{\_}{D})
				}{*}
			})
		}{D}
	}{
		\app{
			(\fun{x}{D})
		}{D}
	}
}
\end{mathpar}

Step 4:

\begin{mathpar}
\ir{D-App$_3$}{
	\val{D}
}{
	\varnothing
	\vdash
	\steps{
		\app{
			(\fun{x}{D})
		}{D}
	}{D}
}
\end{mathpar}

The semantics for the let statement are as follows:

\begin{mathpar}
\ir{D-Let$_1$}{
	\dynJ{\ctx, x\rightarrow e_1}{\steps{e_2}{e_2'}}
}{
	\dynJC{
		\steps{
			\text{let }x=e_1\text{ in }e_2
		}{
			\text{let }x=e_1\text{ in }e_2'
		}
	}
}

\ir{D-Let$_2$}{
	\val{e_2}
}{
	\dynJC{
		\steps{
			\text{let }x=e_1\text{ in }e_2
		}{e_2}
	}
}
\end{mathpar}

\end{document}
